tests/layeff/LowParseWriters.Parsers.fsti
@@ -71,7 +71,7 @@ val deref
 
 inline_for_extraction
 val start
-  (#p: parser)
+  (p: parser)
   (w: LP.leaf_writer_strong (get_serializer p) {
     (get_parser_kind p).LP.parser_kind_high == Some (get_parser_kind p).LP.parser_kind_low
   })
@@ -82,13 +82,23 @@ val start
 inline_for_extraction
 val append
   (#fr: parser)
-  (#p: parser)
+  (p: parser)
   (w: LP.leaf_writer_strong (get_serializer p) {
     (get_parser_kind p).LP.parser_kind_high == Some (get_parser_kind p).LP.parser_kind_low
   })
   (#l: memory_invariant)
   (x: dfst p)
 : Write unit fr (fr `star` p) (fun _ -> True) (fun w _ (w', x') -> w' == w /\ x' == x) l
+
+inline_for_extraction
+val access
+  (p1 p2: parser)
+  (#lens: LP.clens (dfst p1) (dfst p2))
+  (#inv: memory_invariant)
+  (#g: LP.gaccessor (get_parser p1) (get_parser p2) lens)
+  (a: LP.accessor g)
+  (x: ptr p1 inv)
+: Read (ptr p2 inv) (lens.LP.clens_cond (deref_spec x)) (fun res -> lens.LP.clens_cond (deref_spec x) /\ deref_spec res == lens.LP.clens_get (deref_spec x)) inv
 
 val valid_synth_parser_eq
   (p1: parser)
